\documentclass{article}
\begin{document}
\begin{eqnarray*}
uf0(x,y)&=&exp(1)\\
uf1(x)(x,y)&=&exp(x)\\
uf2(x,y)(x,y)&=&exp(x+y)\\
\tau_{{\mathrm{bar}}}&=&0\\
\mathrm{foo}_{1}&=&0\\
\mathrm{bar}_{2^{3}}&=&0\\
\mathrm{bar}&=&0\\
a&=&0\\
A&=&0\\
\mathrm{foo}&=&\mathrm{bar}\\
d&=&\frac{ t }{1}\\
c&=&\mathrm{}( t )\\
\mathrm{uf0}&=&\mathrm{uf0}()\\
p&=&\arcsin\left( 1 \right)\\
s&=&\left(7\right)!\\
r&=&\left( 1 \right)\%\\
q&=&\arctan\left(\infty \right)\\
\mathrm{polygamma}&=&\psi^{\left(0\right)}\left( t \right)\\
o&=&\arccos\left( 0 \right)\\
m&=&\ln\left( e \right)\\
n&=&\cos\left(\pi \right)\\
\mathrm{gamma}&=&\Gamma\left( t \right)\\
\mathrm{Repay}&=&\frac{\mathrm{foo}+\tau_{{\mathrm{bar}}}}{\mathrm{Loans}+ t }\\
\mathrm{catching}&=&\exp\left(\left(\mathrm{Loans}+ t -\left(\mathrm{foo}+\tau_{{\mathrm{bar}}}\right)\right)\times b\right)\\
l&=&\left(1-\theta\left(0.5-\max\left(\theta\left(\theta\left(\mathrm{Repay}- t \right)+\delta\left( t -\mathrm{Repay}\right)-0.5\right),\theta\left(\theta\left( t \right)\right)\right)\right)\right)+\theta\left(\theta\left( t \right)-0.5\right)+\theta\left(\theta\left( t \right)-0.5\right)\\
k&=&\theta\left(\theta\left( t \right)-0.5\right)\theta\left(\theta\left( t \right)+\delta\left( t \right)-0.5\right)+0+0\\
g&=&\left| t \right|\times \mathrm{frac}( t )\times \left\lfloor t \right\rfloor)\times \theta\left(- t \right)\times \theta\left( t \right)\times \theta\left(\mathrm{Repay}- t \right)\times \theta\left(- t \right)+\delta\left( t \right)\times \theta\left( t \right)+\delta\left( t \right)\times \theta\left(\mathrm{Repay}- t \right)+\delta\left( t -\mathrm{Repay}\right)\\
h&=&\delta\left( t \right)+\delta\left( t \right)+\delta\left(g- t \right)\\
i&=&\min\left(g, t \right)\\
j&=&\max\left(g, t \right)+\max\left( t ,0\right)+\min\left( t ,0\right)+\min\left( t ,0\right)+\max\left( t ,0\right)\\
\mathrm{uf1}&=&\mathrm{uf1(x)}\left(j\right)\\
\mathrm{uf2}&=&\mathrm{uf2(x,y)}\left(j,l\right)\\
F(0)&=&0\\
\frac{ d F}{dt} &=&\mathrm{foo}\times  t \\
\mathrm{Loans}(0)&=&0\\
\frac{ d \mathrm{Loans}}{dt} &=&A+\mathrm{Repay}-\mathrm{catching}\\
b(0)&=&-0\\
\frac{ d b}{dt} &=&\mathrm{Repay}-\mathrm{catching}\\
\mathrm{fooey}(0)&=&0\\
\frac{ d \mathrm{fooey}}{dt} &=&\left(a+b\right)^{\log_{d}\left(c\right)}\\
\mathrm{int}(0)&=&0\\
\frac{ d \mathrm{int}}{dt} &=&\tanh\left(\cosh\left(\sinh\left(\tan\left(\cos\left(\sin\left(\ln\left(\sqrt{ t }\right)\right)\right)\right)\right)\right)\right)\\
\mathrm{int1}(0)&=&0\\
\frac{ d \mathrm{int1}}{dt} &=&\arctan\left(\arccos\left(\arcsin\left( t \right)\right)\right)\\
\end{eqnarray*}
\end{document}
